working on stack machine example

Stlc/SM.v
@@ -7,15 +7,39 @@ Require Import Stlc.Stlc_inf.
 Notation open e a := (open_exp_wrt_exp e a).
 
 
+(*************************************************************)
+(*   Connection to nominal representation of terms           *)
+(*************************************************************)
 
-Definition Heap := list (atom * exp).
+(* A named representation of STLC terms.
+   No debruijn indices, and binders include the names of free variables. *)
 
-Inductive StackElem : Set :=
-| ApplyTo : exp -> StackElem.
+Inductive n_exp : Set :=
+ | n_var (x:var)
+ | n_abs (x:var) (e:n_exp)
+ | n_app (e1:n_exp) (e2:n_exp).
 
-Definition Conf := (Heap * exp * list StackElem)%type.
+(* We can rename variables *)
+Definition swap_var (x:var) (y:var) (z:var) : var :=
+  if (z == x) then y else if (z == y) then x else z.
+Fixpoint swap (x:var) (y:var) (e:n_exp) : n_exp :=
+  match e with
+  | n_var z => n_var (swap_var x y z)
+  | n_abs z e => n_abs (swap_var x y z) (swap x y e)
+  | n_app e1 e2 => n_app (swap x y e1) (swap x y e2)
+  end.
 
-Definition initConf (e : exp) : Conf := (nil,e,nil).
+
+(* An abstract machine for named terms *)
+
+Definition heap := list (atom * n_exp).
+
+Inductive frame : Set :=
+| n_app2 : n_exp -> frame.
+
+Definition conf := (heap * n_exp * list frame)%type.
+
+Definition initconf (e : n_exp) : conf := (nil,e,nil).
 
 (* The semantics *)
 
@@ -23,46 +47,40 @@ Inductive Step a := Error   : Step a
                  | Done     : Step a
                  | TakeStep : a -> Step a.
 
-Definition isVal (e : exp) :=
+Definition isVal (e : n_exp) :=
   match e with
-  | abs _ => true
-  | _     => false
+  | n_abs _ _ => true
+  | _         => false
   end.
 
-Definition isTrivial (e: exp) :=
-  match e with
-  | var_f _ => true
-  | _       => false
-end.
 
 
 
-Definition machine_step (c : Conf) : Step Conf := match c with (heap, e, stack) =>
+
+
+Definition machine_step (c : conf) : Step conf :=
+  match c with (heap, e, stack) =>
   match isVal e with
   | true => match stack with
                | nil => Done _
-       (*      | Update v :: stack' => TakeStep (updateOnHeap v e heap, e, stack') *)
-               | ApplyTo a :: stack' =>
+               | n_app2 a :: stack' =>
                  match e with
-                 | abs e =>
-                   match isTrivial a with
-                   | true => TakeStep _ (heap, open e a, stack')
-                   | false =>   let (fresh,_) := atom_fresh (dom heap) in
-                              TakeStep _ ((fresh, a):: heap,
-                                        open e (var_f fresh), stack')
-                   end
+                 | n_abs x e =>
+(*                   match a with
+                   | n_var y => TakeStep _ (heap, swap x y e, stack')
+                   | _     => *)
+                     let (fresh,_) := atom_fresh (dom heap) in
+                     TakeStep _ ((fresh, a):: heap, swap x fresh e, stack')
+(*                    end *)
                  | _ => Error _ (* non-function applied to argument *)
                  end
                end
   | false  =>  match e with
-            | var_f v => match get v heap with
+            | n_var x => match get x heap with
                       | Some e => TakeStep _ (heap, e, stack)
-                      (*          if isVal e
-                    then TakeStep (heap, e, stack)
-                    else TakeStep (heap, e, Update v :: stack) *)
                       | Nothing => Error _ (* Unbound variable *)
                       end
-            | app e1 e2 => TakeStep _ (heap, e1, ApplyTo e2 :: stack)
+            | n_app e1 e2 => TakeStep _ (heap, e1, n_app2 e2 :: stack)
             | _ => Error _ (* should be unreachable (value in nonValueStep) *)
             end
   end
@@ -72,47 +90,172 @@ end.
 (*
 Example run (may take extra steps):
 
-      {}, (\y. (\x. x) y) 0 , nil                     (\y. (\x. x) y) 0
-  ==> {}, (\y. (\x. x) y), ApplyTo 0 :: nil           (\y. (\x. x) y) 0
-  ==> {y -> 0}, (\x.x) y, nil                         (\x. x) 0
-  ==> {y -> 0}, (\x.x), ApplyTo y :: nil              (\x. x) 0
-  ==> {y -> 0}, y , nil                               0
-  ==> {y -> 0}, 0 , nil                               0
+      {}, (\y. (\x. x) y) 0 , nil                  (\y. (\x. x) y) 0
+  ==> {}, (\y. (\x. x) y), app2 0 :: nil           (\y. (\x. x) y) 0
+  ==> {y -> 0}, (\x.x) y, nil                      (\x. x) 0
+  ==> {y -> 0}, (\x.x), app2 y :: nil              (\x. x) 0
+  ==> {y -> 0}, y , nil                            0
+  ==> {y -> 0}, 0 , nil                            0
   ==> Done
 
-decode {y -> 0}, (\x.x), ApplyTo y :: nil
-  == apply_heap { y -> 0 } (apply_stack (ApplyTo y :: nil) (\x.x)
-  == (ApplyTo 0 :: nil) (\x.x)
+decode {y -> 0}, (\x.x), app2 y :: nil
+  == apply_heap { y -> 0 } (apply_stack (app2 y :: nil) (\x.x)
+  == (app2 0 :: nil) (\x.x)
   == (\x.x) 0
 
 *)
 
+(* ------------------------------------------- *)
 
+(* Translation from machine configurations to LN terms *)
 
-Fixpoint apply_stack (s : list StackElem) e :=
+Fixpoint nom_to_exp (ne : n_exp) : exp :=
+  match ne with
+  | n_var x => var_f x
+  | n_app e1 e2 => app (nom_to_exp e1) (nom_to_exp e2)
+  | n_abs x e1 => abs (close_exp_wrt_exp x (nom_to_exp e1))
+end.
+
+Inductive decoded_frame :=
+  | app2 : exp -> decoded_frame.
+
+Fixpoint  decode_stack (s : list frame) : list decoded_frame :=
+  match s with
+  | nil => nil
+  | n_app2 e :: s' => app2 (nom_to_exp e) :: decode_stack s'
+  end.
+
+Fixpoint apply_stack (s : list decoded_frame) (e :exp) : exp :=
   match s with
   | nil => e
-  | ApplyTo e' :: s' => apply_stack s' (app e e')
+  | app2 e' :: s' => apply_stack s' (app e e')
   end.
 
-Lemma app_cong : forall s e e',
-    step e e' ->
-    step (apply_stack s e) (apply_stack s e').
-Proof.
-  induction s.
-  intros; simpl. auto.
-  intros; simpl.
-  destruct a.
-  apply IHs.
-  econstructor. admit.
-  auto.
-Admitted.
-
-Fixpoint apply_heap (h : Heap) e  :=
+(* Note: this is exp -> exp because that is where substitution
+   is defined *)
+Fixpoint apply_heap (h : heap) (e : exp) : exp  :=
   match h with
   | nil => e
-  | (x , e') :: h' => apply_heap h' (subst_exp e' x e)
+  | (x , e') :: h' => apply_heap h' (subst_exp (nom_to_exp e') x e)
   end.
+
+
+Definition decode (c:conf) : exp  :=
+  match c with
+  | (h,e,s) => apply_heap h (apply_stack (decode_stack s) (nom_to_exp e))
+  end.
+
+(* -----------------------------------------  *)
+
+Lemma nom_to_exp_lc : forall ne, lc_exp (nom_to_exp ne).
+Proof.
+  induction ne; simpl; auto.
+  eapply lc_abs_exists with (x1 := x).
+  rewrite open_exp_wrt_exp_close_exp_wrt_exp.
+  auto.
+Qed.
+
+Hint Resolve nom_to_exp_lc : lngen.
+
+Lemma apply_heap_lc : forall h e,
+    lc_exp e ->
+    lc_exp (apply_heap h e).
+Proof.
+  induction h; simpl.
+  auto.
+  intros; destruct a as [y e0].
+  eauto with lngen.
+Qed.
+
+Hint Resolve apply_heap_lc : lngen.
+
+
+
+Lemma decode_lc : forall c, lc_exp (decode c).
+Proof.
+  intro c.
+  destruct c as [[h e] s].
+  simpl.
+  eauto with lngen.
+Admitted.
+
+(* ------------------------------------------ *)
+
+Definition swap_atoms x y S :=
+  if AtomSetImpl.mem x S then
+    if AtomSetImpl.mem y S then S
+    else (add y (AtomSetImpl.remove x S))
+  else
+    if AtomSetImpl.mem y S then
+      (add x (AtomSetImpl.remove y S))
+    else
+      S.
+
+Lemma commute_remove : forall x y S, remove x (remove y S) [=] remove y (remove x S).
+intros. fsetdec.
+Qed.
+
+
+Lemma fv_swap_fresh : forall x0 x (h : heap) n0
+ (Fr1 : x0 `notin` dom h)
+ (SE : remove x (fv_exp (nom_to_exp n0)) [<=] dom h),
+  fv_exp (nom_to_exp (swap x x0 n0)) [<=] add x0 (dom h).
+Proof.
+  induction n0; intros; simpl in *.
+  + unfold swap_var.
+    destruct (x1== x). subst. fsetdec.
+    destruct (x1 == x0). subst. fsetdec.
+    fsetdec.
+  + rewrite fv_exp_close_exp_wrt_exp in *.
+    unfold swap_var.
+    destruct (x1 == x). subst.
+    rewrite IHn0; auto. fsetdec. fsetdec.
+    destruct (x1 == x0). subst.
+    rewrite IHn0; auto. fsetdec.
+    rewrite commute_remove in SE.
+    admit.
+    rewrite IHn0; auto. fsetdec.
+    admit.
+Abort.
+
+Lemma fv_swap_var : forall x y z,
+    singleton (swap_var x y z) [=] swap_atoms x y (singleton z).
+Proof.
+  intros x y z.
+  unfold swap_var, swap_atoms.
+  destruct (z == x).
+  subst.
+Admitted.
+
+Lemma fv_swap : forall x y e,
+    fv_exp (nom_to_exp (swap x y e)) [<=] {{x}} \u {{y}} \u fv_exp (nom_to_exp e).
+Proof.
+  induction e.
+  - simpl.
+    unfold swap_var.
+    destruct (x0 == x). subst. fsetdec.
+    destruct (x0 == y). subst. fsetdec.
+    fsetdec.
+  - simpl.
+    rewrite fv_exp_close_exp_wrt_exp.
+    rewrite IHe.
+    rewrite fv_exp_close_exp_wrt_exp.
+    unfold swap_var.
+    destruct (x0 == x). subst.
+    admit.
+    destruct (x0 == y). subst.
+    admit.
+    fsetdec.
+  - simpl.
+    rewrite IHe1.
+    rewrite IHe2.
+    fsetdec.
+Admitted.
+
+(* ------------------------------------------ *)
+
+(* Since the heap is just an iterated substitution,
+   it inherits properties from subst. *)
 
 Lemma apply_heap_abs : forall h e,
   apply_heap h (abs e) = abs (apply_heap h e).
@@ -128,59 +271,58 @@ Proof.
 Qed.
 
 Lemma apply_heap_open : forall h e e0,
+    lc_exp e0 ->
     apply_heap h (open e e0)  = open (apply_heap h e) (apply_heap h e0).
 Proof.
-  induction h; intros; simpl.
-  auto.
-  destruct a.
-  rewrite subst_exp_open_exp_wrt_exp.
-  rewrite IHh.
-  eauto.
-  admit. (* LC *)
-Admitted.
-
-Fixpoint apply_heap_stack h s :=
-  match s with
-  | nil => nil
-  | ApplyTo a::s' => ApplyTo (apply_heap h a) :: apply_heap_stack h s'
-  end.
-
-Lemma apply_heap_apply_stack : forall h s e,
-      apply_heap h (apply_stack s e) =
-      apply_stack (apply_heap_stack h s) (apply_heap h e).
-Proof.
-  induction s; intros; try destruct a; simpl in *; eauto.
-  rewrite IHs. rewrite apply_heap_app. auto.
+  induction h; intros; simpl; eauto.
+  destruct a; eauto.
+  rewrite subst_exp_open_exp_wrt_exp; eauto with lngen.
 Qed.
+
+
+(* ------------------------------------------ *)
 
 
 Lemma push :
   forall s e e',
-    apply_stack s (app (abs e) e') =
-    apply_stack (ApplyTo e' :: s) (abs e).
+    apply_stack s (app e e') =
+    apply_stack (app2 e' :: s) e.
 simpl. auto.
 Qed.
 
 Lemma combine : forall h x e e',
-  apply_heap h ([x ~> e] e') = (apply_heap ((x,e)::h) e').
+  apply_heap h ([x ~> nom_to_exp e] e') = (apply_heap ((x,e)::h) e').
 Proof.
   simpl. auto.
 Qed.
 
-Fixpoint fv_heap  (h : Heap) :=
-  match h with nil => {} | (x,e) :: h => fv_exp e \u fv_heap h end.
+(* ------------------------------------------ *)
 
 
-Inductive scoped_heap : Heap -> Prop :=
+Fixpoint fv_stack s :=
+  match s with
+    nil => {}
+  | n_app2 e :: s => fv_exp (nom_to_exp e) \u fv_stack s
+  end.
+
+Inductive scoped_heap : heap -> Prop :=
   | scoped_nil  : scoped_heap nil
   | scoped_cons : forall x e h,
       x `notin` dom h ->
-      fv_exp e [<=] dom h ->
+      fv_exp (nom_to_exp e) [<=] dom h ->
       scoped_heap h ->
       scoped_heap ((x,e)::h).
 
+
+Fixpoint fv_heap  (h : heap) :=
+  match h with
+  | nil => {}
+  | (x,e) :: h => fv_exp (nom_to_exp e) \u fv_heap h
+  end.
+
 Lemma scoped_heap_fv_heap_dom : forall h,
-    scoped_heap h -> fv_heap h [<=] dom h.
+    scoped_heap h ->
+    fv_heap h [<=] dom h.
 Proof.
   induction h.
   simpl. fsetdec.
@@ -209,13 +351,11 @@ Proof.
   fsetdec.
 Qed.
 
-Fixpoint fv_stack s :=
-  match s with nil => {} | ApplyTo e :: s => fv_exp e \u fv_stack s end.
 
 Lemma scoped_get : forall h x e,
   scoped_heap h ->
   get x h = Some e ->
-  fv_exp e [<=] dom h.
+  fv_exp (nom_to_exp e) [<=] dom h.
 Proof.
   intros.
   apply scoped_heap_fv_heap_dom in H.
@@ -236,8 +376,8 @@ Qed.
 
 Lemma machine_is_scoped: forall h e s h' e' s',
     machine_step (h,e,s) = TakeStep _ (h',e',s') ->
-    scoped_heap h /\ fv_exp e [<=] dom h /\ fv_stack s [<=] dom h ->
-    scoped_heap h' /\ fv_exp e' [<=] dom h' /\ fv_stack s [<=] dom h.
+    scoped_heap h  /\ fv_exp (nom_to_exp e)  [<=] dom h  /\ fv_stack s [<=] dom h ->
+    scoped_heap h' /\ fv_exp (nom_to_exp e') [<=] dom h' /\ fv_stack s' [<=] dom h'.
 Proof.
   intros.
   simpl in H.
@@ -245,24 +385,25 @@ Proof.
   destruct (isVal e) eqn:?.
   destruct s eqn:?.
   - inversion H.
-  - destruct s0 eqn:?.
+  - destruct f eqn:?.
      + destruct e eqn:?; try solve [inversion H].
-       destruct (isTrivial e0) eqn:?.
-       ++ destruct e0; inversion Heqb0.
-          inversion H; subst; clear H; split; auto.
+(*     destruct n eqn:?.
+       ++ inversion H; subst; clear H; split; auto.
           simpl in *.
-          rewrite fv_exp_open_exp_wrt_exp_upper.
-          simpl.
-          split; fsetdec.
-       ++ destruct (atom_fresh (dom h)).
+          rewrite fv_exp_close_exp_wrt_exp in SE.
+          split.
+          admit.
+          fsetdec.
+       ++ *)
+          destruct (atom_fresh (dom h)).
           inversion H; subst; clear H.
           simpl in *.
-          split. econstructor; eauto. fsetdec.
           split.
-          rewrite fv_exp_open_exp_wrt_exp_upper.
-          simpl.
+            econstructor; eauto. fsetdec.
+          split.
+            rewrite fv_exp_close_exp_wrt_exp in *.
+            admit.
           fsetdec.
-          auto.
   - destruct e eqn:?; try solve [inversion H].
     destruct (get x h) eqn:?;
     inversion H; subst; clear H.
@@ -273,8 +414,11 @@ Proof.
     + simpl in *.
     inversion H; subst; clear H.
     split; auto.
-    split; fsetdec.
-Qed.
+    split; try fsetdec.
+    simpl. fsetdec.
+Admitted.
+
+(* --------------------------------------------------------------- *)
 
 Lemma apply_heap_fresh_eq : forall x e1 h e,
     x `notin` dom h ->
@@ -288,11 +432,27 @@ Proof.
   rewrite (subst_exp_fresh_eq e); auto.
 Qed.
 
+
+
+Fixpoint apply_heap_stack h s :=
+  match s with
+  | nil => nil
+  | app2 a::s' => app2 (apply_heap h a) :: apply_heap_stack h s'
+  end.
+
+Lemma apply_heap_apply_stack : forall h s e,
+      apply_heap h (apply_stack s e) =
+      apply_stack (apply_heap_stack h s) (apply_heap h e).
+Proof.
+  induction s; intros; try destruct a; simpl in *; eauto.
+  rewrite IHs. rewrite apply_heap_app. auto.
+Qed.
+
 Lemma apply_heap_stack_fresh_eq : forall s x e1 h ,
     scoped_heap h ->
     x `notin` dom h ->
     fv_stack s [<=] dom h ->
-    apply_heap_stack ((x, e1) :: h) s = apply_heap_stack h s.
+    apply_heap_stack ((x, e1) :: h) (decode_stack s) = apply_heap_stack h (decode_stack s).
 Proof.
   induction s; intros; simpl; eauto.
   simpl in H.
@@ -303,10 +463,11 @@ Proof.
   fsetdec.
 Qed.
 
+
 Lemma apply_heap_var : forall h x e1,
     x `notin` dom h ->
     x `notin` fv_heap h ->
-    (apply_heap ((x, e1) :: h) (var_f x)) = apply_heap h e1.
+    (apply_heap ((x, e1) :: h) (var_f x)) = apply_heap h (nom_to_exp e1).
 Proof. induction h; intros; simpl.
        destruct (x==x). auto. contradiction.
        destruct a as [y e2].
@@ -319,7 +480,7 @@ Qed.
 Lemma apply_heap_get :  forall h x e,
     scoped_heap h ->
     get x h = Some e ->
-    apply_heap h (var_f x) = apply_heap h e.
+    apply_heap h (var_f x) = apply_heap h (nom_to_exp e).
 Proof.
   induction 1.
   intros; simpl in *. inversion H.
@@ -335,16 +496,26 @@ Proof.
   auto.
 Qed.
 
-Definition decode (c:Conf) : exp :=
-  match c with
-  | (h,e,s) => apply_heap h (apply_stack s e)
-  end.
+
+Lemma app_cong : forall s e e',
+    step e e' ->
+    step (apply_stack s e) (apply_stack s e').
+Proof.
+  induction s.
+  intros; simpl. auto.
+  intros; simpl.
+  destruct a.
+  apply IHs.
+  econstructor. admit.
+  auto.
+Admitted.
+
 
 (* Could be zero steps! *)
 Lemma simulate_step : forall h e s h' e' s' e0 e0',
     machine_step (h,e,s) = TakeStep _ (h',e',s') ->
     scoped_heap h ->
-    fv_exp e [<=] dom h ->
+    fv_exp (nom_to_exp e) [<=] dom h ->
     fv_stack s [<=] dom h ->
     e0 = decode (h,e,s) ->
     e0' = decode (h',e',s') ->
@@ -355,9 +526,9 @@ Proof.
   destruct (isVal e) eqn:?.
   destruct s eqn:?.
   - inversion H.
-  - destruct s0 eqn:?.
+  - destruct f eqn:?.
      + destruct e eqn:?; try solve [inversion H].
-       destruct (isTrivial e1).
+(*       destruct (isTrivial e1).
        ++ inversion H; subst; clear H.
           simpl in *.
           right.
@@ -370,13 +541,15 @@ Proof.
           econstructor.
           admit. (* LC *)
           admit. (* LC *)
-       ++ subst. destruct (atom_fresh).
-          inversion H; subst; clear H.
-          right.
-          simpl in *.
-          rewrite combine.
-          rewrite apply_heap_apply_stack.
-          rewrite apply_heap_apply_stack.
+       ++ *)
+       subst. destruct (atom_fresh).
+       inversion H; subst; clear H.
+       right.
+       simpl in *.
+       rewrite combine.
+
+       rewrite apply_heap_apply_stack.
+       rewrite apply_heap_apply_stack.
 
           rewrite apply_heap_app.
           rewrite apply_heap_abs.
@@ -384,7 +557,9 @@ Proof.
           rewrite apply_heap_stack_fresh_eq; auto; try fsetdec.
           apply app_cong.
 
-          rewrite apply_heap_open.
+          simpl.
+          admit.
+(*          rewrite apply_heap_open.
           rewrite apply_heap_var; eauto.
 
           rewrite apply_heap_fresh_eq.
@@ -395,7 +570,7 @@ Proof.
           auto.
           auto.
           apply scoped_heap_fv_heap_dom in H0.
-          fsetdec.
+          fsetdec. *)
   - destruct e eqn:?; try solve [inversion H].
     destruct (get x h) eqn:?; try solve [inversion H].
     + inversion H; subst; clear H.
@@ -413,9 +588,9 @@ Admitted.
 Lemma simulate_done : forall h e s,
     machine_step (h,e,s) = Done _ ->
     scoped_heap h ->
-    fv_exp e [<=] dom h ->
+    fv_exp (nom_to_exp e) [<=] dom h ->
     fv_stack s [<=] dom h ->
-    is_value e.
+    is_value (nom_to_exp e).
 Proof.
   intros.
   simpl in *.
@@ -423,10 +598,8 @@ Proof.
   destruct s eqn:?.
   - destruct e; simpl in Heqb; inversion Heqb.
     econstructor; eauto.
-  - destruct s0 eqn:?.
+  - destruct f eqn:?.
      + destruct e eqn:?; try solve [inversion H].
-       destruct (isTrivial e0).
-       econstructor; eauto.
        econstructor; eauto.
   - destruct e; inversion H.
     simpl in Heqb. destruct (get x h); inversion H.
